steel/Learn.Steel.ListP.Test.fst
@@ -1,0 +1,40 @@
+module Learn.Steel.ListP.Test
+
+module L   = FStar.List.Pure
+module U32 = FStar.UInt32
+
+open Steel.Effect
+open Steel.Reference
+
+open Learn.Steel.ListP
+
+#push-options "--__no_positivity"
+noeq
+type cell0 = {
+  next: ref cell0;
+  data_x: U32.t;
+  data_y: bool
+}
+#pop-options
+
+inline_for_extraction noextract
+let p0 : list_param =
+  list_param_of_vptr cell0 (U32.t & bool)
+    ({get = (fun c -> c.next); set = (fun c x -> {c with next = x})})
+    (fun c   -> (c.data_x, c.data_y))
+
+let rec p0_length (r : ref cell0)
+  : Steel  U32.t
+          (mlistN p0 r) (fun _ -> mlistN p0 r)
+          (requires fun h0        -> L.length (sel_listN p0 r h0) <= FStar.UInt.max_int U32.n)
+          (ensures  fun h0 len h1 -> frame_equalities (mlistN p0 r) h0 h1 /\
+                                  U32.v len = L.length (sel_listN p0 r h0))
+  = length_body p0 p0_length r
+
+noextract
+let p0_reverse (r : ref cell0)
+  : Steel (ref cell0)
+          (mlistN p0 r) (fun rt -> mlistN p0 rt)
+          (requires fun _ -> True)
+          (ensures fun h0 rt h1 -> sel_listN p0 rt h1 == L.rev (sel_listN p0 r h0))
+  = reverse p0 r
