steel/Learn.Steel.QueueP.Data.fst
@@ -1,0 +1,79 @@
+module Learn.Steel.QueueP.Data
+
+module G  = FStar.Ghost
+module US = Learn.Steel.Util
+
+open Steel.Effect.Common
+open Steel.Effect.Atomic
+open Steel.Reference
+
+open Learn.Steel.ListP.Param
+open Learn.Steel.ListP.Derived
+
+
+let mqueue_vp1 (p : list_param) (q_st : queue_st p.r)
+  : vprop
+  = mlistN p q_st.q_exit
+
+unfold let mqueue_vp (p : list_param) (q : queue_t p)
+  : vprop
+  = vptr q `vdep` mqueue_vp1 p
+
+let mqueue_ref (p : list_param) (q : queue_t p) ((|q_st, l|) : normal (t_of (mqueue_vp p q)))
+  : prop
+  = q_st.q_entry == last_cell p l
+
+let mqueue_rew (p : list_param) (q : queue_t p) ((|_, l|) : normal (t_of (mqueue_vp p q)))
+  : list (cell_t p)
+  = l
+
+unfold let mqueue0 (p : list_param) (q : queue_t p)
+  : vprop
+  = mqueue_vp p q
+       `vrefine`  mqueue_ref p q
+       `vrewrite` mqueue_rew p q
+
+let mqueue_sl p q =
+  let VUnit r = mqueue0 p q in r.hp
+
+let mqueue_sel p q =
+  let VUnit r = mqueue0 p q in r.sel
+
+let mqueue_def p q : squash (mqueue p q == mqueue0 p q) = ()
+
+let intro_mqueue #opened (p : list_param) (q : queue_t p) (l_entry : ref p.r)
+  : SteelGhost  unit opened
+               (vptr q `star` mlistN p l_entry)
+               (fun () -> mqueue p q)
+               (requires fun h ->
+                 let q_st = sel q h in
+                 q_st.q_exit  == l_entry /\
+                 q_st.q_entry == last_cell p (sel_listN p l_entry h))
+               (ensures fun h0 () h1 ->
+                 sel_queue p q h1 == sel_listN p l_entry h0)
+  =
+    intro_vdep (vptr q) (mlistN p l_entry) (mqueue_vp1 p);
+    intro_vrefine (mqueue_vp p q) (mqueue_ref p q);
+    intro_vrewrite (mqueue_vp p q `vrefine` mqueue_ref p q) (mqueue_rew p q);
+    US.rewrite_vprop (US.eq_sym (mqueue_def p q))
+
+let elim_mqueue #opened (p : list_param) (q : queue_t p)
+  : SteelGhost (G.erased (ref p.r)) opened
+               (mqueue p q)
+               (fun l_entry -> vptr q `star` mlistN p l_entry)
+               (requires fun _ -> True)
+               (ensures fun h0 l_entry h1 ->
+                 let l = sel_listN p l_entry h1 in
+                 sel q h1 == {
+                   q_exit  = l_entry;
+                   q_entry = last_cell p l
+                 } /\
+                 l == sel_queue p q h0)
+  =
+    US.rewrite_vprop (mqueue_def p q);
+    elim_vrewrite (mqueue_vp p q `vrefine` mqueue_ref p q) (mqueue_rew p q);
+    elim_vrefine (mqueue_vp p q) (mqueue_ref p q);
+    let q_st = elim_vdep (vptr q) (mqueue_vp1 p) in
+    let rt   = q_st.q_exit in
+    change_equal_slprop (mlistN p q_st.q_exit) (mlistN p rt);
+    rt
