steel/Learn.Steel.QueueP.Data.fsti
@@ -1,0 +1,128 @@
+module Learn.Steel.QueueP.Data
+
+module L   = FStar.List.Pure
+module G   = FStar.Ghost
+module Mem = Steel.Memory
+
+open Steel.Effect.Atomic
+open Steel.Reference
+
+open Learn.Steel.ListP.Param
+open Learn.Steel.ListP.Derived
+
+noeq
+type queue_st (r : Type) = {
+  q_exit  : ref r;
+  q_entry : ref r;
+}
+
+inline_for_extraction
+type queue_t (p : list_param) = ref (queue_st p.r)
+
+let rec last_cell (p : list_param) (l : list (cell_t p))
+  : Tot (ref p.r) (decreases l)
+  = match l with
+    | []     -> null
+    | [c]    -> c._1
+    | _ :: tl -> last_cell p tl
+
+type mqueue_sel_t (p : list_param) = list (cell_t p)
+
+val mqueue_sl (p : list_param u#0) (q : queue_t p)
+  : Mem.slprop u#1
+
+val mqueue_sel (p : list_param) (q : queue_t p)
+  : selector (mqueue_sel_t p) (mqueue_sl p q)
+
+[@@__steel_reduce__]
+let mqueue' (p : list_param) (q : queue_t p) : vprop' =
+  {
+    hp  = mqueue_sl    p q;
+    t   = mqueue_sel_t p;
+    sel = mqueue_sel   p q
+  }
+unfold let mqueue (p : list_param) (q : queue_t p) : vprop =
+  VUnit (mqueue' p q)
+
+
+[@@ __steel_reduce__]
+let sel_queue (#vp:vprop) (p : list_param) (q : queue_t p)
+  (h:rmem vp{FStar.Tactics.with_tactic selector_tactic (can_be_split vp (mqueue p q) /\ True)})
+  : GTot (list (cell_t p))
+  = h (mqueue p q)
+
+
+val intro_mqueue (#opened:Mem.inames) (p : list_param) (q : queue_t p) (l_entry : ref p.r)
+  : SteelGhost  unit opened
+               (vptr q `star` mlistN p l_entry)
+               (fun () -> mqueue p q)
+               (requires fun h ->
+                 let q_st = sel q h in
+                 q_st.q_exit  == l_entry /\
+                 q_st.q_entry == last_cell p (sel_listN p l_entry h))
+               (ensures fun h0 () h1 ->
+                 sel_queue p q h1 == sel_listN p l_entry h0)
+
+val elim_mqueue (#opened:Mem.inames) (p : list_param) (q : queue_t p)
+  : SteelGhost (G.erased (ref p.r)) opened
+               (mqueue p q)
+               (fun l_entry -> vptr q `star` mlistN p l_entry)
+               (requires fun _ -> True)
+               (ensures fun h0 l_entry h1 ->
+                 let l = sel_listN p l_entry h1 in
+                 sel q h1 == {
+                   q_exit  = l_entry;
+                   q_entry = last_cell p l
+                 } /\
+                 l == sel_queue p q h0)
+
+
+let rec last_cell_not_null_lem (p : list_param) (l : list (cell_t p))
+  : Lemma (requires Cons? l /\ L.for_all #(cell_t p) (fun c -> not (is_null c._1)) l)
+          (ensures  is_null (last_cell p l) = false)
+          (decreases l)
+  = match l with
+    | [last] -> ()
+    | _ :: tl -> last_cell_not_null_lem p tl
+
+let mqueue_inv_cases (p : list_param) (q_st : queue_st p.r) (l : mqueue_sel_t p) : prop
+  = (q_st.q_exit ==  null /\ q_st.q_entry ==  null /\ l == []) \/
+    (q_st.q_exit =!= null /\ q_st.q_entry =!= null /\ Cons? l)
+
+let mqueue_inv_cases_lem (p : list_param) (q_st : queue_st p.r) (l : mlistN_sel_t p q_st.q_exit)
+  : Lemma (requires q_st.q_entry == last_cell p l /\
+                    L.for_all #(cell_t p) (fun c -> not (is_null c._1)) l)
+          (ensures  mqueue_inv_cases p q_st l)
+  = match l with
+    | []   -> ()
+    | _ :: _ -> last_cell_not_null_lem p l
+
+let elim_mqueue_cases #opened (p : list_param) (q : queue_t p)
+  : SteelGhost (G.erased (ref p.r)) opened
+               (mqueue p q)
+               (fun l_entry -> vptr q `star` mlistN p l_entry)
+               (requires fun _ -> True)
+               (ensures fun h0 l_entry h1 ->
+                 let q_st = sel q h1 in
+                 let l    = sel_listN p l_entry h1 in
+                 q_st == {
+                   q_exit  = l_entry;
+                   q_entry = last_cell p l
+                 } /\
+                 l == sel_queue p q h0 /\
+                 mqueue_inv_cases p q_st l)
+  = 
+    let l_entry = elim_mqueue p q in
+    let q_st = gget (vptr q) in
+    let l    = gget (mlistN p l_entry) in
+    mlistN_cells_not_null p l_entry;
+    mqueue_inv_cases_lem p q_st l;
+    noop ();
+    l_entry
+
+let rec append_last_cell (p : list_param) (sg0 sg1 : list (cell_t p))
+  : Lemma (requires Cons? sg1)
+          (ensures  last_cell p L.(sg0@sg1) == last_cell p sg1)
+          (decreases sg0)
+  = match sg0 with
+  | [] -> () | _ :: tl -> append_last_cell p tl sg1
