steel/Learn.Steel.QueueP.Impl.fst
@@ -1,0 +1,142 @@
+module Learn.Steel.QueueP.Impl
+
+module L = FStar.List.Pure
+module G = FStar.Ghost
+
+open Steel.Effect
+open Steel.Effect.Atomic
+open Steel.Reference
+
+open Learn.Steel.ListP.Param
+open Learn.Steel.ListP.Derived
+open Learn.Steel.ListP.Data
+open Learn.Steel.QueueP.Data
+
+#set-options "--fuel 3 --ifuel 1 --ide_id_info_off"
+
+(* [malloc] *)
+
+inline_for_extraction
+let malloc (p : list_param) ()
+  : Steel (queue_t p)
+          emp (fun q -> mqueue p q)
+          (requires fun _ -> True) (ensures fun _ q h -> sel_queue p q h == [])
+  =
+    (**) intro_mlistN_nil p null;
+    let q = Steel.Reference.malloc #(queue_st p.r) ({q_exit = null; q_entry = null}) in
+    (**) intro_mqueue p q null;
+    return q
+
+(* [free] *)
+
+inline_for_extraction
+let free (p : list_param) (q : queue_t p)
+  : Steel unit
+          (mqueue p q) (fun () -> emp)
+          (requires fun h -> sel_queue p q h == []) (ensures fun _ _ _ -> True)
+  =
+    (**) let l_entry = elim_mqueue_cases p q in
+    Steel.Reference.free q;
+    (**) elim_mlistN_nil p l_entry
+
+(* [is_empty] *)
+
+inline_for_extraction
+let is_empty (p : list_param) (q : queue_t p)
+  : Steel bool
+          (mqueue p q) (fun _ -> mqueue p q)
+          (requires fun _ -> True)
+          (ensures fun h0 b h1 -> frame_equalities (mqueue p q) h0 h1 /\
+                               Nil? (sel_queue p q h0) <==> b)
+  =
+    (**) let l_entry = elim_mqueue_cases p q in
+    let q_st = read q in
+    (**) intro_mqueue p q l_entry;
+    return (is_null q_st.q_exit)
+
+(* [enqueue] *)
+
+(* TODO? L.unsnoc *)
+let rec unsnoc_queue (p : list_param) (l : list (cell_t p))
+  : Pure (list (cell_t p) & cell_t p)
+         (requires Cons? l)
+         (ensures fun (ini, lt) -> l == L.(ini@[lt]) /\ L.length ini == L.length l - 1)
+         (decreases l)
+  = match l with
+    | [lt] -> [], lt
+    | hd :: tl -> let ini,lt = unsnoc_queue p tl in (hd :: ini, lt)
+
+#push-options "--z3rlimit 20"
+inline_for_extraction
+let enqueue (p : list_param) (x : ref p.r) (q : queue_t p)
+  : Steel  unit
+          ((p.cell x).vp `star` mqueue p q) (fun () -> mqueue p q)
+          (requires fun _ -> True)
+          (ensures fun h0 () h1 -> sel_queue p q h1 == L.snoc (sel_queue p q h0, (|x, g_data p x h0|)))
+  =
+    (**) let h0 = get () in
+    (**) let x_cell = G.hide (|x, g_data p x h0|) in
+    (p.cell x).write_next null;
+    (**) intro_mlist_sglt p x null;
+    (**) let l_entry = elim_mqueue_cases p q in
+    let q_st = read q in
+    (**) let l = gget (mlistN p l_entry) in
+    if is_null q_st.q_entry
+    then begin
+      (**) intro_mlistN p x 1;
+      (**) elim_mlistN_nil p l_entry;
+      write q ({q_exit = x; q_entry = x});
+      (**) intro_mqueue p q x
+    end else begin
+      (**) let ini_lt = G.hide (unsnoc_queue p l) in
+      (**) let ini = G.hide (fst ini_lt) in
+      (**) let lt : G.erased (cell_t p) = G.hide (snd ini_lt) in
+      (**) append_last_cell p ini [G.reveal lt];
+      (**) assert (q_st.q_entry == (G.reveal lt)._1);
+      (**) let len = elim_mlistN p l_entry in
+      (**) let lt' = elim_mlist_append p l_entry len (len-1) (0+1) null ini [G.reveal lt] in
+      (**) assert ((G.reveal lt)._1 == G.reveal lt');
+      (**) let nil = elim_mlist_cons p lt' 0 null in
+      (**) elim_mlist_nil p nil null;
+      (**) change_equal_slprop (mlist p l_entry (len-1) lt'          `star` (p.cell          lt').vp)
+      (**)                     (mlist p l_entry (len-1) q_st.q_entry `star` (p.cell q_st.q_entry).vp);
+      (p.cell q_st.q_entry).write_next x;
+      (**) intro_mlist_cons p q_st.q_entry x 1 null;
+      (**) intro_mlist_append p l_entry (len-1) q_st.q_entry (1+1) null;
+      (**) intro_mlistN p l_entry ((len-1)+(1+1));
+      (**) append_last_cell p ini [G.reveal lt; G.reveal x_cell];
+      (**) L.append_assoc ini [G.reveal lt] [G.reveal x_cell];
+      let q_st = read q in
+      write q ({q_st with q_entry = x});
+      (**) intro_mqueue p q l_entry
+    end
+#pop-options
+
+(* [dequeue] *)
+
+inline_for_extraction
+let dequeue (p : list_param) (q : queue_t p)
+  : Steel (ref p.r)
+          (mqueue p q) (fun x -> (p.cell x).vp `star` mqueue p q)
+          (requires fun h0 -> Cons? (sel_queue p q h0))
+          (ensures fun h0 x h1 -> sel_queue p q h0 == (|x, g_data p x h1|) :: sel_queue p q h1)
+  =
+    (**) let l_entry = elim_mqueue_cases p q in
+    let q_st = read q in
+    let rt = q_st.q_exit in
+    (**) change_equal_slprop (mlistN p l_entry) (mlistN p rt);
+    let nxt = listN_next p rt in
+    (**) let h2 = get () in
+    let q_st = read q in
+    write q ({q_st with q_exit = nxt});
+    if is_null nxt then begin
+      (**) mlistN_entry_null_iff p nxt;
+      let q_st = read q in
+      write q ({q_st with q_entry = null});
+      (**) intro_mqueue p q nxt
+    end else begin
+      (**) intro_mqueue p q nxt;
+      (**) let h3 = get () in
+      (**) assert (sel_queue p q h3 == sel_listN p nxt h2)
+    end;
+    return rt
