steel/Learn.Steel.QueueP.Test.fst
@@ -1,0 +1,44 @@
+module Learn.Steel.QueueP.Test
+
+module L = FStar.List.Pure
+module G = FStar.Ghost
+
+open Steel.Effect
+open Steel.Effect.Atomic
+open Steel.Reference
+
+open Learn.Steel.QueueP
+open Learn.Steel.ListP.Test
+
+
+let p0_queue_t = ref (queue_st cell0)
+
+let p0_malloc   = malloc p0
+let p0_free     = free p0
+let p0_is_empty = is_empty p0
+let p0_enqueue  = enqueue p0
+let p0_dequeue  = dequeue p0
+
+
+let test_p0 () : SteelT unit emp (fun () -> emp)
+  =
+    let q = p0_malloc () in
+    let x0 = Steel.Reference.malloc #cell0 ({next = null; data_x = 0ul; data_y = true}) in
+    p0_enqueue x0 q;
+    (**) let x0_c : cell_t p0 = (|x0, (0ul, true)|) in
+    (**) assert_norm (L.snoc ([], x0_c) == [x0_c]);
+    let x1 = Steel.Reference.malloc #cell0 ({next = null; data_x = 1ul; data_y = false}) in
+    p0_enqueue x1 q;
+    let x0' = p0_dequeue q in
+    (**) assert (x0' == x0);
+    let x0_v = read x0' in
+    (**) assert (x0_v.data_x = 0ul /\ x0_v.data_y = true);
+    write x0' ({x0_v with data_x = 2ul});
+    p0_enqueue x0' q;
+    let x1' = p0_dequeue q in
+    (**) assert (x1' == x1);
+    let x0' = p0_dequeue q in
+    (**) assert (x0' == x0);
+    Steel.Reference.free x0';
+    Steel.Reference.free x1';
+    p0_free q
