steel/Learn.Steel.QueueP.fst
@@ -1,0 +1,5 @@
+module Learn.Steel.QueueP
+
+include Learn.Steel.ListP.Param
+include Learn.Steel.QueueP.Data
+include Learn.Steel.QueueP.Impl
